

Задача 1

$$Y = m(X) + \varepsilon, \quad X = (X_1, \dots, X_n)$$

$$Q(a, b) = \sum_{i=1}^n q_n(x) (X_i - x) [Y_i - a(x) - b(x) \cdot (X_i - x)]^2$$

$$\hat{m}(x) = \arg \min_{a(x), b(x)} Q(a, b)$$

$$\begin{cases} \frac{\partial Q}{\partial a} = 0 \\ \frac{\partial Q}{\partial b} = 0 \end{cases}$$

Далее, для краткости,

$$d_i := X_i - x$$

$$w_i := q_n(x) \cdot (X_i - x)$$

$$\frac{\partial Q}{\partial a} = \left[\sum_{i=1}^n w_i (a^2 - 2Y_i a - 2Y_i b d_i + 2a b d_i + Y_i^2 + b^2 d_i^2) \right] \Big|'_a =$$

$$= \sum_{i=1}^n w_i (\cancel{a^2} - \cancel{2} Y_i \cancel{a} - \cancel{2} Y_i b d_i + \cancel{2} a b d_i + Y_i^2 + b^2 d_i^2) = 0 \Rightarrow \textcircled{I} a = \frac{\sum_{i=1}^n w_i (Y_i - b d_i)}{\sum_{i=1}^n w_i}$$

$$\frac{\partial Q}{\partial b} = \sum_{i=1}^n w_i (\cancel{\frac{1}{2}} b d_i^2 + \cancel{\frac{1}{2}} a d_i - \cancel{\frac{1}{2}} Y_i d_i) = 0 \Rightarrow b = \frac{\sum_{i=1}^n w_i d_i (Y_i - a)}{\sum_{i=1}^n w_i d_i^2}$$

$$a = \textcircled{I} = \textcircled{II}$$

$$\textcircled{II} a = \frac{\sum_{i=1}^n w_i d_i (Y_i - b d_i)}{\sum_{i=1}^n w_i d_i}$$

$$\sum_{i=1}^n w_i d_i \cdot \sum_{i=1}^n w_i (Y_i - b d_i) = \sum_{i=1}^n w_i \cdot \sum_{i=1}^n w_i d_i (Y_i - b d_i)$$

$$\sum_{i=1}^n w_i^2 d_i (\cancel{Y_i - b d_i}) + \sum_{i \neq j} w_i w_j d_i (Y_i - b d_j) = \sum_{i=1}^n w_i^2 d_i (\cancel{Y_i - b d_i}) + \sum_{i \neq j} w_i w_j d_j (Y_j - b d_i)$$

$$\sum_{i \neq j} w_i w_j (Y_j (d_i - d_j) - b (d_i d_j - d_j^2)) = 0$$

Отсюда:

$$b = \frac{\sum_{i \neq j} w_i w_j Y_j (d_i - d_j)}{\sum_{i \neq j} w_i w_j d_j (d_i - d_j)}$$

$$a = \frac{\sum_{i=1}^n w_i Y_i - (\sum_{i=1}^n w_i d_i) \cdot \frac{\sum_{i \neq j} w_i w_j Y_j (d_i - d_j)}{\sum_{i \neq j} w_i w_j d_j (d_i - d_j)}}{\sum_{i=1}^n w_i}$$